<section xml:id="sec_function-composition">
  <title>Function Composition</title>
  <introduction>
    <p><idx>composition</idx> Suppose <m>f</m> and <m>g</m> are functions, and that the domain of <m>g</m> contains all real numbers in the range of <m>f</m>.  We can then <sq>chain</sq> the two functions together and get a new function by first evaluating <m>f</m> at <m>x</m>, and then evaluating <m>g</m> at <m>f(x)</m>.  This new function is called the <term>composition</term> of <m>f</m> and <m>g</m>, and is denoted by <m>(g \circ f)</m>.  The formal definition is</p>

    <me>
      (g \circ f)(x) = g(f(x))
    </me>

    <p>As with other functions, the domain of <m>(g\circ f)</m> is taken to be the largest set of real numbers for which the function is defined.  This is the set of all <m>x</m> such that <m>x</m> is in the domain of <m>f</m> and <m>f(x)</m> is in the domain of <m>g</m> (because first <m>f</m> is evaluated at <m>x</m>, and then <m>g</m> is evaluated at <m>f(x)</m>).</p>

    <example>
      <title>Function Composition</title>
      <statement>
        <p>Let <m>f(x) = 3x -1</m> and <m>g(x) = x^2 + 1</m>.  Then:</p>
        <ul>
          <li>
            <m>f(2) = 3(2) -1 = 6-1 = 5</m> and <m>g(2) = 2^2+1 = 4+1 =5</m>.
          </li>
          <li>
            <m>(g \circ f)(2) = g(f(2)) = g(5) = 26</m>.
          </li>
          <li>
            <m>(f \circ g)(2) = f(g(2)) = f(5) = 14</m>.
          </li>
          <li>
            <p>Note: the previous two bullet points imply that <m>(g \circ f)(x)</m> is not necessarily equal to <m>(f \circ g)(x)</m>.  The order in which functions are composed matters!</p>
          </li>
          <li>
            <m>(g\circ f)(y) = g(f(y)) = g(3y-1) = (3y-1)^2 + 1 = 9y^2-6y + 1 + 1 = 9y^2-6y + 2</m>
          </li>
          <li>
            <m>(f\circ g)(x) = f(g(x)) = f(x^2 + 1) = 3(x^2 + 1) - 1 = 3x^2 + 3 -1 = 3x^2 +2</m>
          </li>
          <li>
            <p>Both <m>(g \circ f)</m> and <m>(f \circ g)</m> have domain equal to the set of all real numbers.</p>
          </li>
        </ul>
      </statement>
    </example>

    <example>
      <title>More Function Composition</title>
      <statement>
        <p>Let: <m>f(x)=\sqrt{x+2}</m> and <m>g(x) = {3-x}</m>.  Determine the domain of <m>(g \circ f)</m>, the domain of <m>(f \circ g)</m> and an expression for each of these functions.</p>
      </statement>
      <solution>
        <p>First, note that the domain of <m>f</m> is <m>[-2,\infty)</m>, and the domain of <m>g</m> is the set of all real numbers.</p>
        <p>The domain of <m>(g \circ f)</m> is the set of all <m>x</m> such that <m>x</m> is in the domain of <m>f</m> and <m>f(x)</m> is in the domain of <m>g</m>.  This is <m>[-2,\infty)</m> because <m>x</m> must belong to the domain of <m>f</m>, and since the domain of <m>g</m> is the set of all real numbers, for any such <m>x</m> the number <m>f(x)</m> is in the domain of <m>g</m>.</p>

        <p>We have</p>

        <me>
          \begin{aligned}
            (g \circ f)(x) &amp;= g(f(x)) \\
            &amp;= g(\sqrt{x+2}) \\
            &amp;= 3 - \sqrt{x+2}
          \end{aligned}
        </me>

        <p>The domain of <m>(f \circ g)</m> is the set of all <m>x</m> such that <m>x</m> is in the domain of <m>g</m> and <m>g(x)</m> is in the domain of <m>g</m>.  The domain of <m>g</m> is the set of all real numbers, so now we need to determine which of these are such that <m>g(x) = 3-x</m> is in <m>[-2, \infty)</m>, the domain of <m>f</m>.  This happens when <m>3 - x \geq -2</m>, that is, when <m>x \leq 5</m>.  Therefore the domain of <m>(f \circ g)</m> is <m>(-\infty,5]</m>.</p>

        <p>We have</p>

        <me>
          \begin{aligned}
            (f\circ g)(x) &amp;= f(g(x)) \\
            &amp;= f(3-x) \\
            &amp;= \sqrt{(3-x)+2}=\sqrt{5-x}
          \end{aligned}
        </me>
      </solution>
    </example>

    <p>A skill that is useful in calculus is recognizing when a function can be expressed as a composition of two other functions.</p>

    <example>
      <title>Recognizing Function Composition</title>
      <statement>
        <p>Suppose <m>h(x) = (x^3-1)^7+2</m>.  Find functions <m>f</m> and <m>g</m> such that <m>h = (g \circ f)</m>.</p>
      </statement>
      <solution>
        <p>Looking at the expression of <m>h(x)</m>, it is an expression raised to the power 7, plus 2.  Thus it makes sense to take <m>f(x)</m> to be that expression, i.e., <m>f(x) = x^3 - 1</m>, and <m>g(x)</m> to be a function that raises its input to the seventh power and then adds two, i.e., <m>g(x) = x^7 + 2</m>.</p>

        <p>As a check, we can compute</p>

        <me>
          \begin{aligned}
            (g \circ f)(x) &amp;= g(f(x)) \\
            &amp;= g(x^3 - 1) \\
            &amp;= (x^3-1)^7+2 \\
            &amp;= h(x)
          \end{aligned}
        </me>
      </solution>
    </example>
  </introduction>
  <exercises>
    <title>Practice Problems</title>
    <exercise>
      <statement>
        <p>Let <m>f(x)=3x+5</m>, <m>g(x) = \frac{x^2+1x+2}{x}</m> and <m>h(x)=\sqrt{x+7}</m>.</p>
        <ol>
          <li>
            <p>Find a formula for <m>(f\circ g)(x)</m>.  What is the domain of <m>(f\circ g)(x)</m>?</p>
          </li>
          <li>
            <p>Find a formula for <m>(g\circ f)(x)</m>.  What is the domain of <m>(g\circ f)(x)</m>?</p>
          </li>
          <li>
            <p>Find a formula for <m>(f\circ h)(x)</m> .What is the domain of <m>(f\circ h)(x)</m>?</p>
          </li>
          <li>
            <p>Find a formula for <m>(h\circ f)(x)</m>.  What is the domain of <m>(h\circ f)(x)</m>?</p>
          </li>
          <li>
            <p>Find a formula for <m>(h\circ g)(x)</m>. What is the domain of <m>(h\circ g)(x)</m>?</p>
          </li>
        </ol>
      </statement>
      <answer>
        <ol>
          <li>
            <p>
              <m>(f\circ g)(x)=\frac{3x^2+8x+6}{x}</m>, Domain: <m>\{x:x\neq 0\}</m>.
            </p>
          </li>
          <li>
            <p>
              <m>(g\circ f)(x)=\frac{9x^2+33x+32}{3x+5}</m>, Domain: <m>\{x:x\neq -\frac{5}{3}\}</m>.
            </p>
          </li>
          <li>
            <p>
              <m>(f\circ h)(x)=3\sqrt{x+7}+5</m>, Domain: <m>\{x:x\geq-7\}</m>.
            </p>
          </li>
          <li>
            <p>
              <m>(h\circ f)(x)=\sqrt{3x+12}</m>, Domain: <m>\{x:x\geq-4\}</m>.
            </p>
          </li>
          <li>
            <p>
              <m>(h\circ g)(x)=\sqrt{\frac{x^2+1x+2}{x}+7}</m>, Domain: <m>\{x:-4-\sqrt{14}\leq x\leq\sqrt{14}-4</m> or <m>x>0\}</m>.
            </p>
          </li>
        </ol>
      </answer>
    </exercise>
    <exercise>
      <statement>
        <p>Let <m>f(x)=\sqrt{x}</m> and <m>g(x)=x^2</m>.</p>
        <ol>
          <li>
            <p>Find a formula for <m>(f\circ g)(x)</m>.  What us the domain of <m>(f\circ g)(x)</m>?</p>
          </li>
          <li>
            <p>Find a formula for <m>(g\circ f)(x)</m>.  What us the domain of <m>(g\circ f)(x)</m>.</p>
          </li>
          <li>
            <p>Do the functions in (a) and (b) have the same domain?  What does this tell you?</p>
          </li>
        </ol>
      </statement>
      <answer>
        <ol>
          <li>
            <p>
              <m>(f\circ g)(x)=\sqrt{x^2}</m>, Domain:<m>(-\infty,\infty)</m>.
            </p>
          </li>
          <li>
            <p>
              <m>(g\circ f)(x)=(\sqrt{x})^2</m>, Domain:<m>[0,\infty)</m>.
            </p>
          </li>
          <li>
            <p>They are not the same, and therefore the two functions are not the same.</p>
          </li>
        </ol>
      </answer>
    </exercise>
    <exercise>
      <statement>
        <p>Find functions <m>f(x)</m> and <m>g(x)</m> so that <m>(g \circ f)(x) = 3e^{2x-4} + x</m>.</p>
      </statement>
      <answer>
        <p>
          <m>f(x) = 2x-4</m> and <m>g(x) = 3e^x + \frac{x+4}{2}</m>.
        </p>
      </answer>
    </exercise>
  </exercises>
</section>
