<section xml:id="sec_logarithms">
  <title>Logarithms</title>
  <introduction>
    <p><idx>logarithm</idx> From our previous work, we know that if <m>b > 0</m> then the range of the exponential function <m>f(x) = b(x)</m> is the positive real numbers.  If <m>b > 0</m> then the graph of <m>f</m> increases as we move right on the <m>x</m> axis, and if <m>0 \lt b \lt 1</m> then it increases as we move left on the <m>x</m>-axis. (The function <m>f(x) = b^x</m> is not very exciting if <m>b = 1</m>.) In either case, that means for any positive real number <m>y</m> there exists a unique real number <m>x</m> such that <m>b^x = y</m>.  This number is <term>the base-<m>b</m> logarithm of <m>y</m></term>, and denoted by <m>\log_b(y)</m>.  That is, if <m>b > 0</m> and <m>b \neq 1</m>, then <m>\log_b(y)</m> is the power to which <m>b</m> must be raised in order to get the positive number <m>y</m>.</p>

    <p>It is important to notice that <m>\log_b(y)</m> is only defined for positive numbers <m>y</m>.  Logarithms are exponents.  By definition <m>b^{\log_b(y)} = y</m>.  Since <m>b</m> is positive, so is any power of <m>b</m>.  Thus <m>\log_b(y)</m> is undefined when <m>y</m> is negative because no power of a positive number can give us a negative number.</p>

    <p>Logarithms have properties that follow immediately from the fact that they are exponents.</p>

    <p><em>Properties of Logarithms</em>.  Suppose <m>b > 0</m> and <m>b \neq 1</m>.</p>

    <ul>
      <li>
        <p>
          <m>\log_b{1} = 0</m> because <m>b^0 = 1</m>.
        </p>
      </li>
      <li>
        <p>
          <m>\log_b{b} = 1</m> because <m>b^1 = b</m>.
        </p>
      </li>
      <li>
        <p>
          <m>b^x = y</m> if and only if <m>\log_b(y) = x</m>.
        </p>
      </li>
      <li>
        <p>
          <m>\log_b(xy) = \log_b(x) + \log_b(y)</m> because <m>b^{\log_b(x) + \log_b(y)} = b^{log_b(x)} b^{\log_b(y)} = xy</m>.
        </p>
      </li>
      <li>
        <p>
          <m>\log_b(a^x) = x \log_b(a)</m> because <m>b^{x \log_b(a)} = \left(b^{\log_b(a)}\right)^x = a^x</m>.
        </p>
      </li>
      <li>
        <p>
          <m>\log_b\left(\frac{x}{y}\right) = \log_b(x) - \log_b(y)</m> because <m>b^{ \log_b(x) - \log_b(y)} = b^{log_b(x)} b^{-\log_b(y)} = b^{log_b(x)} \cdot \frac{1}{b^{\log_b(y)}} = \frac{x}{y}</m>.
        </p>
      </li>
    </ul>

    <p><idx>common logarithms</idx><idx>natural logarithms</idx> When the base <m>b</m> is omitted, as in <m>\log(100)</m>, it is assumed to be 10.  Logarithms to base 10 are called <em>common logarithms</em>.  Logarithms to base <m>e</m> are called <em>natural logarithms</em>, and denoted by <m>ln(x)</m> rather than <m>log_e(x)</m>.</p>

    <example>
      <title>Evaluating Logarithms</title>
      <statement>
        <p>
          Evaluate each expression.
          <ul>
            <li>
              <p>
                <m>\log_2{(2)} = 1</m>
              </p>
            </li>
            <li>
              <p>
                <m>\log{(100)} = \log{(10^2)} = \log_{10}{(10^2)} = 2</m>
              </p>
            </li>
            <li>
              <p>
                <m>\log_{6}{(12)} + \log_{6}{(18)} = \log_{6}{(12 \cdot 18)} = \log_{6}{(216)} = \log_{6}{(6^3)} = 3</m>
              </p>
            </li>
            <li>
              <p>
                <m>\log_{5}{(2500)} - \log_{5}{(4)} = \log_{5}{(\frac{2500}{4})} = \log_{5}{(625)} = \log_{5}{(5^4)} = 4</m>
              </p>
            </li>
            <li>
              <p>
                <m>\log(5b) + \log(2c^2) = \log(10bc^2) = \log(10) + \log(bc^2) = 1 + \log(bc^2)</m>
              </p>
            </li>
          </ul>
        </p>
      </statement>
    </example>

    <example>
      <title>Solving Equations with Logarithms</title>
      <statement>
        <p>Solve <m>\log_8(x) + \log_8(x - 12) = 2</m>.</p>
      </statement>
      <solution>
        <p>We have <m>2 = \log_8(x) + \log_8(x - 12) = \log_8(x(x - 12))</m>, so that <m>8^2 = x(x - 12)</m>, by the definition of logarithms.  Thus <m>x^2 - 12 - 64 = 0</m>.  By factoring (or using the quadratic formula first for help), this is the same as <m>(x-16)(x+4) = 0</m>.  Therefore <m>x = 16</m> or <m>x = -4</m>.  But <m>x = -4</m> is not a solution, as <m>\log_8(-4)</m> is undefined.  Hence the solution is <m>x = 16</m>.</p>
      </solution>
    </example>

    <p>For a positive real number <m>b \neq 1</m>, the <em>logarithm function with base <m>b</m></em> is the function <m>f(x) = \log_b(x)</m>. Its domain is the set of positive real numbers.  Its range is the set of all real numbers.</p>

    <p>Notice that the functions <m>f(x) = b^x</m> and <m>g(y) = \log_b(y)</m> are inverses by definition: <m>b^x = y</m> if and only if <m>\log_b(y) = x</m>.  Thus, if <m>b \neq 1</m>, the logarithm function with base <m>b</m> is the inverse of the exponential function with base <m>b</m>. (The function <m>f(x) = 1^x</m> does not have an inverse because, for example <m>1^2 = 1^3 = 1</m>.)</p>

    <p>Finally, we observe that logarithm functions with different bases are just multiples of each other.  We know <m>b^{\log_b(x)} = x</m>.  Therefore, <m>\log_a\left(b^{\log_b(x)}\right) = \log_a(x)</m>.  From one of the properties of logarithms, we know that <m>\log_a\left(b^{\log_b(x)}\right) =\log_b(x) \log_a(b)</m>, and so this is the same as <m>\log_b(x) \log_a(b) = \log_a(x)</m>.  Since <m>\log_a(b)</m> is a number, this says that <m>\log_a(x)</m> is a multiple of <m>\log_b(x)</m>.</p>
    <p>The graphs of <m>f(x) = log(x)</m> and <m>g(x) = \ln(x)</m> are shown below.</p>

    <image>
      <latex-image>
        <![CDATA[
        \begin{tikzpicture}
          \begin{axis}[grid=both, xmax=3.7, ymax=3, axis lines=middle, restrict y to domain=-7:12, enlargelimits]
            \addplot[red, domain=-0.2:3.3,samples=100]  {log10(x)} node[below]{\(f(x) = \log(x)\)};
            \addplot[blue, domain=-0.2:3.3,samples=100]  {ln(x)} node[above]{\(g(x) = \ln(x)\)};
          \end{axis}
        \end{tikzpicture}
        ]]>
      </latex-image>
    </image>

    <p>The same principles as before of shifting graphs or stretching them vertically or horizontally apply.</p>

    <example>
      <title>Graphing Logarithmic Functions</title>
      <statement>
        <p>Sketch the graph of <m>f(x) = 5\log(x+2) + 3</m>.</p>
      </statement>
      <solution>
        <p>This graph has the same basic shape as the graph of <m>y = \log(x)</m>.  It is shifted upwards by 3 and left by 2.  Also, it is stretched in the vertical direction by a factor of 5.</p>

        <p>After plotting a few well chosen points and sketching a curve of the correct shape through them, one arrives at the graph below.</p>

        <image>
          <latex-image>
            <![CDATA[
            \begin{tikzpicture}
              \begin{axis}[grid=both, xmax=6, ymax=7, axis lines=middle, restrict y to domain=-7:12, enlargelimits]
              \addplot[blue,domain=-1.999:6,samples=100]  {5*log10(x+2)} node[above left]{$y=5\log_{10}{(x+2)} + 3$};
              \end{axis}
            \end{tikzpicture}
            ]]>
          </latex-image>
        </image>
      </solution>
    </example>
  </introduction>
  <exercises>
    <title>Practice Problems</title>
    <statement>
      <p>In questions 1 to 5, use the properties of logarithms to to find an equivalent, arguably simpler, expression.</p>
    </statement>
    <exercise>
      <statement>
        <m>\log_{6}{(12)} + \log_{6}{(18)}</m>
      </statement>
      <answer>
        <m>3</m>
      </answer>
    </exercise>
    <exercise>
      <statement>
        <m>\log_8(x) + \log_8(x - 12)</m>
      </statement>
      <answer>
        <m>\log_{8}{(x^2-12x)}</m>
      </answer>
    </exercise>
    <exercise>
      <statement>
        <m>\log_{5}{(2500)} - \log_{5}{(4)}</m>
      </statement>
      <answer>
        <m>4</m>
      </answer>
    </exercise>
    <exercise>
      <statement>
        <m>\log(5b) + \log(2c^2)</m>
      </statement>
      <answer>
        <m>\log(10bc^2)</m>
      </answer>
    </exercise>
    <exercise>
      <statement>
        <m>\log_{25}{(7)} + \log_5{(3)}</m>
      </statement>
      <answer>
        <m>\frac{2\log{(3)}+\log{(7)}}{2\log{(5)}}</m>
      </answer>
    </exercise>
    <exercise>
      <statement>
        <p>Sketch the graph of <m>h(x)=1-5\log{(1-\frac{x}{2})}</m>.</p>
      </statement>
      <answer>
        <image>
          <latex-image>
            <![CDATA[
            \begin{tikzpicture}
              \begin{axis}[grid=both, xmax=10, ymax=7, axis lines=middle, enlargelimits]
                \addplot[blue, domain=-50:10]  {1-(5*log10(1-(x/2)))} node[left]{\(h(x)=1-5\log{(1-\frac{x}{2})}\)};
              \end{axis}
            \end{tikzpicture}
            ]]>
          </latex-image>
        </image>
      </answer>
    </exercise>
  </exercises>
</section>
