<section xml:id="sec_rational-exponents">
  <title>Rational Exponents</title>
  <introduction>
    <p><idx>rational exponent</idx> For a real number <m>x</m> and positive integers <m>m</m> and <m>n</m> , we define <m>x^{\frac{m}{n}}</m> to be the real number <m>y</m> such that <m>y^n = x^m</m>, if such a number <m>y</m> exists.  Notice how this coincides with the definition of exponents <m>\frac{1}{n}</m> when <m>m = 1</m>.</p>

    <example>
      <title>Working out Rational Exponents</title>
      <statement>
        <ul>
          <li>
            <p>
              <m>9^\frac{1}{2} = 3</m> because <m>3^2 = 9^1</m>
            </p>
          </li>
          <li>
            <p>
              <m>8^\frac{2}{3} = 4</m> because <m>4^3 = 64 = 8^2</m>
            </p>
          </li>
          <li>
            <p>
              <m>(-3)^\frac{5}{2}</m> is undefined since <m>(-3)^5 = -243</m> and a negative number is not the square of any number (because <m>y^2 \geq 0</m> for every real number <m>y</m>).
            </p>
          </li>
        </ul>
      </statement>
    </example>

    <p>It follows from the definition that</p>

    <me>x^\frac{m}{n} = \left(x^m\right)^\frac{1}{n}</me>

    <p>and, if <m>x^\frac{1}{n}</m> is defined, then</p>

    <me>x^\frac{m}{n} = \left(x^\frac{1}{n}\right)^m</me>

    <example xml:id="ex2">
      <title>Rational Exponents Read Both Ways</title>
      <statement>
        <ul>
          <li>
            <p>
              <m>5^\frac{3}{2} = \left(5^3\right)^\frac{1}{2} = \sqrt{125}</m>.  Also <m>5^\frac{3}{2} = \left(5^\frac{1}{2}\right)^3 = \left(\sqrt{5}\right)^3 = \sqrt{125}</m>.  Note that <m>\left(\sqrt{5}\right)^3 = \sqrt{125}</m> because squaring both sides gives 125.
            </p>
          </li>
          <li>
            <p>
              <m>\left(-3\right)^\frac{6}{2} = \left(\left(-3\right)^6\right)^\frac{1}{2} = \sqrt{729} = 27</m>, but <m>\left(\left(-3\right)^\frac{1}{2}\right)^6</m> is undefined because <m>\left(-3\right)^\frac{1}{2}</m> is undefined.
            </p>
          </li>
        </ul>
      </statement>
    </example>

    <p>When a rational exponent is not in lowest terms, for example as in the last bullet point of <xref ref="ex2">Example</xref>, it is tempting to reduce it to lowest terms.  Care is needed, however, because that can be a terrible idea.  Using that same example, <m>\left(-3\right)^\frac{6}{2} = 27</m>, but <m>\left(-3\right)^3 = -27</m>.  Hence <m>\left(-3\right)^\frac{6}{2} \neq \left(-3\right)^3</m> even though <m>\frac{6}{2} = 3</m>.  Why?  It is a question of applying the definition properly.  The difficulty is that <m>(-3)^6</m> is positive, so that <m>\left(-3\right)^\frac{6}{2} = \left(\left(-3\right)^6\right)^\frac{1}{2}</m> is positive, but <m>\frac{6}{2} = 3</m> is an odd integer and a negative number raised to an odd power is negative.  When reducing a rational exponent to lowest terms, one should always check whether the expression obtained has the same sign as the original expression.  This issue only arises when the base is negative.</p>

    <p>The familiar rules of exponents apply to expressions involving rational exponents.  When exponential expressions with the same base are multiplied, the exponents are added, as in</p>

    <me>2^\frac{2}{3} 2^\frac{4}{5} = 2^{\frac{2}{3} + \frac{4}{5}} = 2^\frac{22}{15}</me>

    <p>Note that all numbers involved in positive, so each equality holds.  When an exponential expression is raised to a higher power, the exponents are multiplied as in</p>

    <me>\left((-3)^3\right)^\frac{2}{5} = (-3)^\frac{6}{5}</me>

    <p>Both the left hand side and right hand side of this statement are positive, so the equality holds.</p>

    <example>
      <title>Working with Rational Exponents</title>
      <statement>
        <ul>
          <li>
            <p>Look at <m>8^\frac{2}{3} = (8^2)^\frac{1}{3}=(64)^\frac{1}{3}=4</m>.  Since <m>8^\frac{1}{3}</m> is defined, we can also compute <m>(8^\frac{1}{3})^2 = 2^2 = 4</m>.</p>
          </li>
          <li>
            <p>
              Look at <m>625^\frac{3}{4} = (625^3)^\frac{1}{4}=(244140625)^\frac{1}{4}=125</m>.  Since <m>625^\frac{1}{4}</m> is defined, we can also compute <m>(625^\frac{1}{4})^3 = 5^3 = 125</m>, which is arguably an easier calculation.
            </p>
          </li>
          <li>
            <p>
              Look at <m>(-49)^\frac{4}{2} = \left((-49)^4\right)^\frac{1}{2} = \sqrt{(-49)^4} = \sqrt{5764801} = 2401</m>.  We can not compute as <m>\left((-49)^\frac{1}{2}\right)^4</m> because <m>(-49)^\frac{1}{2}</m> is not defined.  We can compute as <m>(-49)^\frac{4}{2} = (-49)^2 = 2401</m> because <m>(-49)^\frac{4}{2}</m> is positive (because <m>(-49)^4</m> is positive) and so is <m>(-49)^2</m>.
            </p>
          </li>
          <li>
            <p>
              Look at <m>(-5)^\frac{10}{2} = \sqrt{(-5)^{10}} = \sqrt{25^5} = \left(\sqrt{25}\right)^5 = 5^5</m>.  We can not compute as <m>\left((-5)^\frac{1}{2}\right)^{10}</m> because <m>(-5)^\frac{1}{2}</m> is undefined.  And in this case, since <m>(-5)^{10}</m> is positive we have that <m>(-5)^\frac{10}{2}</m> is positive, whereas <m>(-5)^5</m> is negative, so <m>(-5)^\frac{10}{2} \neq (-5)^5</m>.
            </p>
          </li>
        </ul>
      </statement>
    </example>

    <p>Finally, as before,</p>

    <me>
      \begin{aligned}
        x^{-\frac{m}{n}} &amp;= \left(x^{-1}\right)^\frac{m}{n} \\
        &amp;= \left(\frac{1}{x}\right)^\frac{m}{n} \\
        &amp;= \left(\left(\frac{1}{x}\right)^m\right)^\frac{1}{n} \\
        &amp;= \left(\frac{1}{x^m}\right)^\frac{1}{n}
        &amp;= \frac{1}{x^\frac{m}{n}}
      \end{aligned}
    </me>

    <p>when <m>x^{-\frac{m}{n}}</m> is defined.</p>

    <example>
      <title>Finding a Base Given a Rational Exponent</title>
      <statement>
        <p>Find <m>x</m> if <m>x^\frac{3}{5} = -7</m>.</p>
      </statement>
      <solution>
        <p>Since <m>x^\frac{3}{5} = -7</m>, we have that <m>x^3 = \left(x^\frac{3}{5}\right)^5 = (-7)^5</m>, so that</p>
        <me>
          x = \left(x^3\right)^\frac{1}{3} = \left((-7)^5\right)^\frac{1}{3} = (-7)^\frac{5}{3}
        </me>
      </solution>
    </example>
  </introduction>
  <exercises>
    <title>Practice Problems</title>
    <statement><p>In questions 1 to 5, find a simpler form of each expression.</p></statement>
    <exercise>
      <statement>
        <m>-16^\frac{3}{2}</m>
      </statement>
      <answer>
        <m>-64</m>
      </answer>
    </exercise>
    <exercise>
      <statement>
        <m>(\frac{8}{343})^{-\frac{2}{3}}</m>
      </statement>
      <answer>
        <m>\frac{49}{4}</m>
      </answer>
    </exercise>
    <exercise>
      <statement>
        <m>(27)^\frac{5}{3}</m>
      </statement>
      <answer>
        <m>243</m>
      </answer>
    </exercise>
    <exercise>
      <statement>
        <m>(-6)^{\frac{6}{2}}</m>
      </statement>
      <answer>
        <m>216</m>
      </answer>
    </exercise>
    <exercise>
      <statement>
        <m>(-\frac{32}{243})^\frac{2}{5}</m>
      </statement>
      <answer>
        <m>\frac{4}{9}</m>
      </answer>
    </exercise>
    <exercise>
      <statement>
        <p>Find <m>x</m> if <m>x^{\frac{7}{4}} = 9</m>.</p>
      </statement>
      <answer>
        <m>9^\frac{4}{7} = 3^\frac{8}{7}</m>
      </answer>
    </exercise>
  </exercises>
</section>
